io/case-studies/TC.MLify.MIIO.fst
@@ -34,6 +34,14 @@ instance mlifyable_miio
 (** Ideas to improve this:
 1. The initial function should be t1 -> IIO t2 pi.
 2. What if instead of Tot, we use Ex, to be able to internalize try_catch.
+   This implies writing a lift from Ex to IIOwp. To do that, we also have to 
+   write elim_ex (similar to elim_pure). I did not try to write it yet.
+   But what does exactly means to use Ex? 
+   Why Ex and not another effect? Answer: well, Ex has native extraction,
+     therefore the try_with block will be extracted to the OCaml's native
+     try/with.
+   Maybe to not create more confusion & to not tie things too much to F*,
+   it is better to not use Ex since it may be just a hack (check with Catalin).
 3. 
 
 **)
@@ -44,8 +52,8 @@ instance mlifyable_tot_miio
   mk_mlifyable
     #((t1 -> Tot t2) -> MIIO t3) #(trivial_MIIO (t1 -> Tot t2) _) #(weak_tot_miio t1 t2 t3)
     ((t1 -> Tot t2) -> ML t3)
-    (fun f x -> admit ();
-     let tree : iio t2 = reify (f x) [] (fun _ _ -> True) in
+    (fun f x ->
+     let tree : iio t3 = reify (f x) [] (fun _ _ -> True) in
      match tree with
      | Return y -> y
      (** during extraction, Free.IO.Call is replaced with an actual
